New examples to test JUMPI rule

example/CFGExamples.thy
@@ -100,4 +100,158 @@ apply (rule impI)
 apply(sep_cancel)+
 done
 
+(* Same example but we put an unknown value and an if in the post condition *)
+(* For a jumpif where we don't know at all which branch to follow, it works *)
+definition c2 where
+"c2 x = build_cfg [ Stack (PUSH_N [x]), Stack (PUSH_N [8]), Pc JUMPI, Stack (PUSH_N [1]), Misc STOP, Pc JUMPDEST, Stack (PUSH_N [2]), Misc STOP]"
+
+schematic_goal c2_val:
+ " c2 x = ?p"
+apply(simp add: c2_def word_rcat_simps Let_def evm_fun_simps dropWhile.simps  cfg_simps next_i_def concat_map_def
+  split:if_splits nat.splits option.splits )
+done
+
+lemma
+notes if_split[ split del ]
+shows
+ " triple_cfg (c2 cond)
+(continuing ** stack_height 0 ** program_counter (0,0) ** gas_pred 1000)
+(the (cfg_blocks (c2 cond) 0))
+(if word_rcat [cond] = (0::256 word) then stack 0 (word_rcat [2::byte]) else stack 0 (word_rcat [1::byte]) )
+"
+apply(unfold c2_val)
+apply (simp)
+apply(rule cfg_jumpi)
+ apply(simp)
+ apply(simp)
+ apply(simp)
+apply(rule seq_inst)
+apply(rule inst_strengthen_pre[OF inst_push_n[where rest=emp]])
+ apply(rule impI)
+ apply(sep_cancel)+
+ apply(simp add: gas_pred_def)
+ apply(rule conjI; clarsimp)
+ apply(simp)
+ apply(simp)
+apply(rule seq_inst)
+apply(rule inst_strengthen_pre[OF inst_push_n[where rest="stack 0 (word_rcat [cond])" 
+      and h="Suc 0"]])
+ apply(rule impI)
+ apply(sep_cancel)+
+ apply(simp add: program_counter_def)
+apply(rule seq_jumpi)
+ apply(rule impI)
+ apply (sep_select 5)
+apply(sep_cancel)+
+apply (subst sep_emp)
+apply (simp add: program_counter_def)
+apply(rule conjI; clarsimp)
+ apply(simp)
+apply(simp)
+apply(simp)
+apply(rule cfg_no)
+apply(rule seq_inst)
+apply(rule inst_strengthen_pre[OF inst_jumpdest[where g="(1000 - 2 * Gverylow - Ghigh)" and h="0" and rest=emp]])
+ apply(rule impI)
+ apply(sep_cancel)+
+ apply(simp add: gas_pred_def)
+apply(rule seq_inst)
+apply(rule inst_strengthen_pre[OF inst_push_n[where h="0" and rest=emp and g="(1000 - 2 * Gverylow - Ghigh - Gjumpdest)"]])
+ apply(rule impI)
+ apply(sep_cancel)+
+ apply(simp add: program_counter_def)
+apply(rule seq_inst)
+apply(rule inst_strengthen_pre[OF inst_stop[where h="Suc 0" and rest="stack 0 (word_rcat [2]) \<and>* gas_pred (1000 - 2 * Gverylow - Ghigh - Gjumpdest -
+          Gverylow)"]])
+ apply(rule impI)
+ apply(sep_cancel)+
+ apply(simp add: program_counter_def)
+ apply(simp)
+apply(rule seq_strengthen_pre[OF seq_no[where rest="not_continuing \<and>* action (ContractReturn []) \<and>* 
+      stack_height (Suc 0) \<and>* program_counter (8, 3) \<and>* gas_pred (1000 - 2 * Gverylow - Ghigh - Gjumpdest - Gverylow)"]])
+apply (rule impI)
+apply(sep_cancel)+
+apply(simp)
+apply(rule cfg_no)
+apply(rule seq_inst)
+apply(rule inst_strengthen_pre[OF inst_push_n[where h="0" and rest=emp and g="(1000 - 2 * Gverylow - Ghigh)"]])
+ apply(rule impI)
+ apply(sep_cancel)+
+ apply(simp add: gas_pred_def)
+apply(rule seq_inst)
+apply(rule inst_strengthen_pre[OF inst_stop[where h="Suc 0" and rest="stack 0 (word_rcat [1]) \<and>* gas_pred (1000 - 2 * Gverylow - Ghigh -
+          Gverylow)"]])
+ apply(rule impI)
+ apply(sep_cancel)+
+ apply(simp add: program_counter_def)
+ apply(simp)
+apply(rule seq_strengthen_pre[OF seq_no[where rest="not_continuing \<and>* action (ContractReturn []) \<and>* 
+      stack_height (Suc 0) \<and>* program_counter (5, 2) \<and>* gas_pred (1000 - Ghigh - 3 * Gverylow)"]])
+apply (rule impI)
+apply(sep_cancel)+
+done
+
+(* Same example as the previous one but with the unknown value as a precondition *)
+definition c3 where
+"c3 x = build_cfg [ Stack (PUSH_N [x]), Stack (PUSH_N [8]), Pc JUMPI, Stack (PUSH_N [1]), Misc STOP, Pc JUMPDEST, Stack (PUSH_N [2]), Misc STOP]"
+
+schematic_goal c3_val:
+ " c3 x = ?p"
+apply(simp add: c3_def word_rcat_simps Let_def evm_fun_simps dropWhile.simps  cfg_simps next_i_def concat_map_def
+  split:if_splits nat.splits option.splits )
+done
+
+lemma
+notes if_split[ split del ]
+shows
+ " triple_cfg (c3 cond)
+(continuing ** stack_height 0 ** program_counter (0,0) ** gas_pred 1000 **
+ \<langle> (word_rcat [cond] \<noteq> (0::256 word)) \<rangle>)
+(the (cfg_blocks (c3 cond) 0))
+(stack 0 (word_rcat [1::byte]) )
+"
+apply(unfold c3_val)
+apply (simp)
+apply(rule cfg_jumpi[where rest="\<langle>word_rcat [cond] \<noteq> (0::256 word)\<rangle>"])
+ apply(simp)
+ apply(simp)
+ apply(simp)
+apply(rule seq_inst)
+apply(rule inst_strengthen_pre[OF inst_push_n[where rest="\<langle>word_rcat [cond] \<noteq> (0::256 word)\<rangle>"]])
+ apply(rule impI)
+ apply(sep_cancel)+
+ apply(simp )
+apply(rule seq_inst)
+apply(rule inst_strengthen_pre[OF inst_push_n[where rest="stack 0 (word_rcat [cond]) \<and>* \<langle>word_rcat [cond] \<noteq> (0::256 word)\<rangle>" 
+      and h="Suc 0"]])
+ apply(rule impI)
+ apply(sep_cancel)+
+ apply(simp add: program_counter_def)
+apply(rule seq_jumpi)
+ apply(rule impI)
+ (* apply (sep_select 8) *)
+apply(sep_cancel)+
+apply (simp)
+apply(simp)
+apply(simp)
+apply(rule cfg_false_pre)
+
+apply(rule cfg_no)
+apply(rule seq_inst)
+apply(rule inst_strengthen_pre[OF inst_push_n[where h="0" and rest=emp and g="(1000 - 2 * Gverylow - Ghigh)"]])
+ apply(rule impI)
+ apply(sep_cancel)+
+ apply(simp add: gas_pred_def)
+apply(rule seq_inst)
+apply(rule inst_strengthen_pre[OF inst_stop[where h="Suc 0" and rest="stack 0 (word_rcat [1]) \<and>* gas_pred (1000 - 2 * Gverylow - Ghigh -
+          Gverylow)"]])
+ apply(rule impI)
+ apply(sep_cancel)+
+ apply(simp add: program_counter_def)
+ apply(simp)
+apply(rule seq_strengthen_pre[OF seq_no])
+apply (rule impI)
+apply(sep_cancel)+
+done
+
 end
